src/hint/hint_sem_aux_void.v
@@ -1,4 +1,4 @@
-Require Import vgtac.
+Require Import sflib.
 
 Require Import vellvm.
 Require Import hint_sem.
