src/proceed/hint_sem_props_proceed_call.v
@@ -1,4 +1,4 @@
-Require Import vgtac.
+Require Import sflib.
 Require Import vellvm.
 Require Import memory_sim.
 Require Import genericvalues_inject.
@@ -22,7 +22,7 @@ Import Opsem.
 Import syntax_ext.
 Import hints.
 
-Definition retval_update st rid rv : (@Opsem.ECStack DGVs) :=
+Definition retval_update st rid rv : (Opsem.ECStack) :=
   match st with
     | nil => st
     | ec::ecs => 
@@ -109,7 +109,7 @@ Proof.
   destruct Haincr as [Haincr _]; eapply gv_inject_incr; eauto.
 Qed.
 
-Definition update_olc_by_ocmd olc lc ocmd : @GVsMap DGVs :=
+Definition update_olc_by_ocmd olc lc ocmd : GVsMap :=
   match ocmd with
     | ret cmd =>
       match (vars_aux.def_cmd cmd) with
