src/proceed/hint_sem_props_proceed_maydiff.v
@@ -1,4 +1,4 @@
-Require Import vgtac.
+Require Import sflib.
 Require Import vellvm.
 Require Import memory_sim.
 Require Import genericvalues_inject.
