Makefile
@@ -1,0 +1,49 @@
+COQMODULE     := LLVMBerry
+COQDEFINITION := $(wildcard src/validator/*.v)
+COQEXTRACT    := $(wildcard src/extraction/*.v)
+COQPROOF      := $(filter-out $(COQEXTRACT), $(filter-out $(COQDEFINITION), $(wildcard src/*/*.v)))
+COQTHEORIES   := $(COQDEFINITION) $(COQEXTRACT) $(COQPROOF)
+
+.PHONY: all vellvm
+
+all: proof
+
+init:
+	git submodule init
+	git submodule update
+	$(MAKE) -C lib/vellvm init
+	cd lib/llvm; git submodule init; git submodule update
+
+Makefile.coq: Makefile $(COQTHEORIES)
+	(echo "-R src $(COQMODULE)"; \
+   echo "-R lib/sflib sflib"; \
+   echo "-R lib/paco/src Paco"; \
+   echo "-R lib/vellvm/src Vellvm"; \
+   echo "-R lib/vellvm/lib/metalib metalib"; \
+   echo "-R lib/vellvm/lib/cpdtlib Cpdt"; \
+   echo "-R lib/vellvm/lib/compcert-2.4 compcert"; \
+   echo $(COQTHEORIES)) > _CoqProject
+	coq_makefile -f _CoqProject -o Makefile.coq
+
+lib: lib/sflib lib/paco/src lib/vellvm
+	$(MAKE) -C lib/sflib
+	$(MAKE) -C lib/paco/src
+	$(MAKE) -C lib/vellvm
+
+definition: Makefile.coq lib $(COQDEFINITION)
+	$(MAKE) -f Makefile.coq $(patsubst %.v,%.vo,$(COQDEFINITION))
+
+proof: definition $(COQPROOF)
+	$(MAKE) -f Makefile.coq $(patsubst %.v,%.vo,$(COQPROOF))
+
+extract: definition $(COQEXTRACT)
+	$(MAKE) -C lib/vellvm extract
+	$(MAKE) -C src/extraction clean
+	$(MAKE) -C src/extraction
+
+%.vo: Makefile.coq
+	$(MAKE) -f Makefile.coq "$@"
+
+clean: Makefile.coq
+	$(MAKE) -f Makefile.coq clean
+	rm -f Makefile.coq
