README.md
@@ -3,50 +3,43 @@
 ## Development ##
 
 ### Requirements ###
+
 - Install OCaml.
     + Install [opam](http://opam.ocamlpro.com/), the right way to install OCaml.
-    + `opam switch 4.01.0 && opam update && opam upgrade`
+    + `opam switch 4.02.3 && opam update && opam upgrade`
     + `opam install menhir ott batteries biniou cppo easy-format yojson ctypes`
 
-- Install [Coq](http://coq.inria.fr/download) from tarball.
-    + IMPORTANT: use have to configure with `./configure -usecamlp4`. The `-usecamlp4` option is required.
-    + After configuration, do `make && sudo make install`
-
-- Install [paco](plv.mpi-sws.org/paco/) library.
-    + `git clone git@github.com:snu-sf/paco.git` somewhere. Command below in `/src`.
-    + `make`
-    + `sudo make install`
+- Install [Coq](http://coq.inria.fr/download) from OPAM.
+    + `opam install coq.8.5.0~camlp4`
 
 - Get [Boost](http://www.boost.org/users/history/version_1_59_0.html) C++ library.
     + Unzip somewhere.
     + Add `export BOOST_ROOT=$BOOST_LOCATION` (or `export BOOST_INCLUDEDIR=$BOOST_LOCATION`) in `.bashrc` or `.zshrc`.   
 
-- Clone the repository.
+### Build ###
 
-- `git submodule init && git submodule update`
-    + If above commands do not work, check format of `url` in `.gitmodules` are start with `https://github.com`.
+- `make init`
+    + It (recursively) downloads submodules.
+    + If above commands do not work, check format of `url` in `.gitmodules` starts with `git@github.com:snu-sf/`.
     + If you meet `permission denied (publickey)` error when perform `git submodule update`, do `git submodule sync` && `git submodule update`
 
-- Build `vellvm`.
-    + See `https://github.com/snu-sf/vellvm-legacy` for more details.
-    + `script/build-vellvm.sh $JOBS`
+- `make lib`
+    + It builds `vellvm-legacy`.  See `https://github.com/snu-sf/vellvm-legacy` for more details.
     + `lib/vellvm/src/` will contain `.vo` files.
-    + `lib/vellvm/` will contain extracted `.ml`, `.mli` files.
+    + `lib/vellvm/src/Extraction` will contain extracted `.ml`, `.mli` files.
 
 - Build `llvm`.
-    + `git submodule init && git submodule update` to install Cereal.
     + `script/build-llvm.sh $JOBS`
     + `.build/llvm-obj` will contain llvm object files.
     + `.local/bin` will contain llvm installation.
 
-### Build ###
-- Move `.coqrc` to `$HOME`. Here, replace $SIMPLBERRY_HOME to your simplberry directory.
-- `make` in `/src`
+- `make`
 
 ### Debugging ###
+
 - For those who participate in this project, there are some useful techniques to track a program flow of validator or identify cause of a bug.
     + `export OCAMLRUNPARAM='b'` lets validator show call stack when it aborts
 
 ### TODO ###
-`src/main.ml`
-- line 70: Currently we don't free memory spaces.
+
+- `src/main.ml:70`: Currently we don't free memory spaces.
